Organized map definitions.

lib/adts/map.bpl
@@ -2,74 +2,81 @@
  * The key-value map ADT.
  */
 
-const unique get, put, contains: Method;
+/**
+ * Exported declarations
+ */
 
+const unique Map.get, Map.put, Map.contains: Method;
+type Map.State = [int] int;
 function Map.key(n: Invoc): int;
 function Map.value(n: Invoc): int;
 
-axiom (forall n: Invoc :: Invoc.name(n) == put ==> Map.key(n) == Invoc.args(n)[0]);
-axiom (forall n: Invoc :: Invoc.name(n) == put ==> Map.value(n) == Invoc.args(n)[1]);
-axiom (forall n: Invoc :: Invoc.name(n) == get ==> Map.key(n) == Invoc.args(n)[0]);
-axiom (forall n: Invoc :: Invoc.name(n) == contains ==> Map.value(n) == Invoc.args(n)[0]);
-
-// A function to restrict a Set to invocations involving key ke
-function restr(s: Set, k: int) returns (t: Set);
-
-// restr is a subset
-axiom (forall s: Set, k: int :: Set.subset(restr(s, k), s));
-
-// restr is monotonic w.r.t subset
-axiom (forall s, t: Set, k: int :: Set.subset(s, t) ==> Set.subset(restr(s, k), restr(t, k)));
-
-// Adding an invocation on k increases restr
-axiom (forall q: Seq, n: Invoc :: {restr(Set.ofSeq(Seq.append(q, n)), Map.key(n))}
-        restr(Set.ofSeq(Seq.append(q, n)), Map.key(n))
-          == Set.add(restr(Set.ofSeq(q), Map.key(n)), n));
-
-// Adding invocations not on k preserves restr
-axiom (forall q: Seq, n: Invoc, k: int :: Map.key(n) != k
-       ==> restr(Set.ofSeq(Seq.append(q, n)), k) == restr(Set.ofSeq(q), k));
-
-type AbsState = [int]int; // Abstract state
-
 // A function to calculate the abstract state after executing a subset vis of
 // a sequence of invocations lin
-function state(vis: Set, lin: Seq) returns (m: AbsState);
+function Map.ofVis(vis: Set, lin: Seq): Map.State;
 
+// TODO define this one directly instead of Map.ofVis
+function Map.ofSeq(seq: Seq): Map.State;
 
-// The effect of appending an invocation on key k on state of k
-axiom (forall s1, s2: Set, q1, q2: Seq, n: Invoc ::
-       q2 == Seq.append(q1, n) && s2 == Set.add(s1, n)
-       ==> (Invoc.name(n) == put ==> state(s2, q2)[Map.key(n)] == Map.value(n)));
-
-// Appending a get/contains invocation does not change state
-axiom (forall s1, s2: Set, q1, q2: Seq, n: Invoc, k: int ::
-       q2 == Seq.append(q1, n) && s2 == Set.add(s1, n)
-       && (Invoc.name(n) == get || Invoc.name(n) == contains)
-       ==> state(s2, q2)[k] == state(s1, q1)[k]);
-
-// The effect of appending an invocation on key k on state with unchanged vis
-axiom (forall s: Set, q1: Seq, n: Invoc, k: int ::
-          state(s, q1)[k] == state(s, Seq.append(q1, n))[k]);
-
-
-// The mapping of key k depends only invocations involving k
-axiom (forall s: Set, q: Seq, k: int ::
-        state(s, q)[k] == state(restr(s, k), q)[k]);
-axiom (forall q: Seq, k: int ::
-        state(Set.ofSeq(q), q)[k] == state(restr(Set.ofSeq(q), k), q)[k]);
-
-// Taking union with a restriction of a super-set means restrictions are same
-axiom (forall s0, s1, t: Set, k: int ::
-        s1 == Set.union(s0, t) && Set.subset(restr(s0, k), t) ==>
-          restr(s1, k) == restr(t, k)
-);
+// A function to Map.restrict a Set to invocations involving key ke
+function Map.restr(s: Set, k: int): Set;
 
 // Union of disjoint keys means state comes from one of the two sets
 procedure {:layer 1} lemma_state_Set.union(k: int, K: int, s, t: Set);
   requires (forall n: Invoc :: Set.elem(n, s) ==> Map.key(n) < k);
   requires (forall n: Invoc :: Set.elem(n, t) ==> k <= Map.key(n));
   ensures (forall i: int :: 0 <= i && i < k ==>
-    state(Set.union(s, t), lin)[i] == state(s, lin)[i]);
+    Map.ofVis(Set.union(s, t), lin)[i] == Map.ofVis(s, lin)[i]);
   ensures (forall i: int :: k <= i && i < K ==>
-    state(Set.union(s, t), lin)[i] == state(t, lin)[i]);
+    Map.ofVis(Set.union(s, t), lin)[i] == Map.ofVis(t, lin)[i]);
+
+/**
+ * Internal declarations
+ */
+
+axiom (forall n: Invoc :: Invoc.name(n) == Map.put ==> Map.key(n) == Invoc.args(n)[0]);
+axiom (forall n: Invoc :: Invoc.name(n) == Map.put ==> Map.value(n) == Invoc.args(n)[1]);
+axiom (forall n: Invoc :: Invoc.name(n) == Map.get ==> Map.key(n) == Invoc.args(n)[0]);
+axiom (forall n: Invoc :: Invoc.name(n) == Map.contains ==> Map.value(n) == Invoc.args(n)[0]);
+
+// Map.restr is a subset
+axiom (forall s: Set, k: int :: Set.subset(Map.restr(s, k), s));
+
+// Map.restr is monotonic w.r.t subset
+axiom (forall s, t: Set, k: int :: Set.subset(s, t) ==> Set.subset(Map.restr(s, k), Map.restr(t, k)));
+
+// Adding an invocation on k increases Map.restr
+axiom (forall q: Seq, n: Invoc :: {Map.restr(Set.ofSeq(Seq.append(q, n)), Map.key(n))}
+        Map.restr(Set.ofSeq(Seq.append(q, n)), Map.key(n))
+          == Set.add(Map.restr(Set.ofSeq(q), Map.key(n)), n));
+
+// Adding invocations not on k preserves Map.restr
+axiom (forall q: Seq, n: Invoc, k: int :: Map.key(n) != k
+       ==> Map.restr(Set.ofSeq(Seq.append(q, n)), k) == Map.restr(Set.ofSeq(q), k));
+
+// The effect of appending an invocation on key k on state of k
+axiom (forall s1, s2: Set, q1, q2: Seq, n: Invoc ::
+       q2 == Seq.append(q1, n) && s2 == Set.add(s1, n)
+       ==> (Invoc.name(n) == Map.put ==> Map.ofVis(s2, q2)[Map.key(n)] == Map.value(n)));
+
+// Appending a get/contains invocation does not change state
+axiom (forall s1, s2: Set, q1, q2: Seq, n: Invoc, k: int ::
+       q2 == Seq.append(q1, n) && s2 == Set.add(s1, n)
+       && (Invoc.name(n) == Map.get || Invoc.name(n) == Map.contains)
+       ==> Map.ofVis(s2, q2)[k] == Map.ofVis(s1, q1)[k]);
+
+// The effect of appending an invocation on key k on state with unchanged vis
+axiom (forall s: Set, q1: Seq, n: Invoc, k: int ::
+          Map.ofVis(s, q1)[k] == Map.ofVis(s, Seq.append(q1, n))[k]);
+
+// The mapping of key k depends only invocations involving k
+axiom (forall s: Set, q: Seq, k: int ::
+        Map.ofVis(s, q)[k] == Map.ofVis(Map.restr(s, k), q)[k]);
+axiom (forall q: Seq, k: int ::
+        Map.ofVis(Set.ofSeq(q), q)[k] == Map.ofVis(Map.restr(Set.ofSeq(q), k), q)[k]);
+
+// Taking union with a Map.restriction of a super-set means Map.restrictions are same
+axiom (forall s0, s1, t: Set, k: int ::
+        s1 == Set.union(s0, t) && Set.subset(Map.restr(s0, k), t) ==>
+          Map.restr(s1, k) == Map.restr(t, k)
+);
